\documentclass[varwidth=70mm]{standalone}
%standard width: 70 mm
\input{preamble}
\excludecomment{answer}
%\includecomment{answer}           
           
\begin{document}
\begin{center}
\begin{asy}
size(50mm);
import markers;
import geometry;

real l = 4, theta = 32.5;
real AB = l*Cos(theta);
pair A = (0,0);
pair B = (AB*Cos(theta), AB*Sin(theta));
pair C = (l,0);
pair D = (2*l*Cos(theta)^2, 2*AB*Sin(theta));
pair E = (2*l*Cos(theta)^2, 0);

draw(A--B--C--cycle);
draw(C--E--D--B--cycle);
draw(A--D, StickIntervalMarker(2, 1, black));

label("$A$", A, SW);
label("$B$", B, NW);
label("$C$", C, S);
label("$D$", D, NE);
label("$E$", E, SE);
label("$l$", (A+C)/2, S);
markangle("$\theta$", radius=10, C, A, B);
perpendicular(B, NE, A-B, size=5);
perpendicular(E, NE, D-E, size=5);
\end{asy}
\end{center}
In the figure, the length of $AC$ is denoted by $l$ ($l>0$) and $\ang{0}<\theta <\ang{90}$. $AB\perp CB$ and $AE\perp DE$. If $AB=BD$, which of the following must be true?
\begin{itemize}
	\item[I.] $\bigtriangleup ABC \sim \bigtriangleup AED$
	\item[II.] area of $\bigtriangleup AED$ is $2l^2\sin\theta\cos^3\theta$
	\item[III.] $CE > 0$ for $\ang{0} < \theta < \ang{45}$
\end{itemize} 

\begin{choices}
\choice I and II only
\choice I and III only
\choice II and III only
\choice I, II and III%
\end{choices}

\begin{answer}
\hrulefill\par
\textbf{Ans: D}

\begin{itemize}
	\item[1.] $\angle ABC = \angle AED = \ang{90}$
	\item[2.] $\angle BAC = \angle EAD = \theta$
	\item[3.] $\angle BCA = \angle EDA = \ang{90}-\theta$
\end{itemize}
By AAA, $\bigtriangleup ABC \sim \bigtriangleup AED$.\par
$\therefore$ I is true.\par\medskip

Area of $\bigtriangleup AED = \frac{1}{2}DE\times AE$
\begin{equation*}
\begin{aligned}[c]
\sin\theta &= \frac{DE}{AD} \\
		   &= \frac{DE}{2AB} \\
\therefore DE &= 2AB\sin\theta
\end{aligned}
\qquad
\begin{aligned}[c]
\cos\theta &= \frac{AE}{AD} \\
		   &= \frac{AE}{2AB} \\
\therefore AE &= 2AB\cos\theta
\end{aligned}
\end{equation*}
Consider  $\bigtriangleup ABC$,
\begin{equation*}
\begin{aligned}
\cos\theta &= \frac{AB}{AC} \\
		   &= \frac{AB}{l} \\
\therefore AB &= l\cos\theta		   
\end{aligned}
\end{equation*}
Combining everything,
\begin{equation*}
\begin{aligned}
\text{Area of }\bigtriangleup AED &= \frac{1}{2}DE\times AE \\
								  &= \frac{1}{2}(2AB\sin\theta)(2AB\cos\theta) \\
								  &= 2AB^2\sin\theta\cos\theta \\
								  &=  2(l\cos\theta)^2\sin\theta\cos\theta \\
								  &= 2l^2\sin\theta\cos^3\theta
\end{aligned}
\end{equation*}
$\therefore$ II is true.\par\medskip

\begin{equation*}
\begin{aligned}
CE &= AE - AC \\
   &= 2AB\cos\theta - AC \\
   &= 2(l\cos\theta)\cos\theta - l \\
   &= l(2\cos^2\theta - 1)
\end{aligned}
\end{equation*}
For $CE > 0$,
\begin{equation*}
\begin{aligned}
l(2\cos^2\theta - 1) &> 0 \\
			\cos\theta &> \frac{1}{\sqrt{2}} \\
\end{aligned}
\end{equation*}
$\theta = \ang{45}$ for $\cos\theta = \frac{1}{\sqrt{2}}$ and $\cos\theta$ is decreasing from $\theta = \ang{0}$ to \ang{90}, so $\theta$ cannot be greater than \ang{45} for $\cos\theta > \frac{1}{\sqrt{2}}$. Since $\ang{0} < \theta < \ang{90}$, so $\ang{0} < \theta < \ang{45}$.\par
$\therefore$ III is true.
\end{answer}

\end{document}