\documentclass[varwidth=70mm]{standalone}
%standard width: 70 mm
\input{preamble}
\excludecomment{answer}
\includecomment{answer}
           
\begin{document}

Let $a_n$ be the $n$-th term of a sequence for any positive integer $n$. If $a_1 = 1$ and $$a_{n+1} = a_n + \frac{1}{a_n}$$ Which of the following must be true?
\begin{itemize}
	\item[I.] $a_1$, $a_2$, $a_3$\ldots form an arithmetic sequence
	\item[II.] $a_4 = \dfrac{29}{10}$
	\item[III.] $a_{2020}^{2} - a_{2019}^{2}  = \dfrac{1}{a_{2019}^{2}} + \dfrac{1}{2}$
\end{itemize} 

\begin{choices}
\choice I only
\choice II only%
\choice I and III only
\choice II and III only
\end{choices}

\begin{answer}
\hrulefill\par
\textbf{Ans: B}

An arithmetic sequence is of the form $a$, $a+d$, $a+2d$\ldots
\begin{equation*}
\begin{aligned}
a_1 &= 1 \\
a_2 &= 1 + \frac{1}{1} \\
	&= 2 \\
a_3 &= 2 + \frac{1}{2} \\
	&= \frac{5}{2}
\end{aligned}
\end{equation*}
$a_2 - a_1 = 2 - 1 = 1$ and $a_3 - a_2 = \frac{5}{2} - 2 = \frac{1}{2}$

$\therefore$ I is false

\begin{equation*}
\begin{aligned}
a_4 &= a_3 + \frac{1}{a_3} \\
	&= \frac{5}{2} + \frac{2}{5} \\
	&= \frac{29}{10}
\end{aligned}
\end{equation*}
$\therefore$ II is true

\begin{equation*}
\begin{aligned}
a_{n+1} &= a_n + \frac{1}{a_n} \\
a_{n+1}^2 &= \left(a_n + \frac{1}{a_n}\right)^2 \\
a_{n+1}^2 &= a_n^2 + \frac{1}{a_n^2} + 2 \\
a_{n+1}^2 - a_n^2 &= \frac{1}{a_n^2} + 2 \\
\end{aligned}
\end{equation*}
For $n=2019$,
\begin{equation*}
\begin{aligned}
a_{2020}^2 - a_{2019}^2 &= \frac{1}{a_{2019}^2} + 2 \\
\end{aligned}
\end{equation*}
$\therefore$ III is false
\end{answer}
\end{document}